ServiceProvider.fst
@@ -12,7 +12,8 @@ let serviceprovider me client idp =
   let reqRes = recieve client in (*1*)
   match reqRes with
   | HttpGet (uri) -> 
-	let (authnReq, sigSP)  = createAuthnRequest me idp in 
+    let (authnReq, sigSP)  = CreateAuthnRequest me idp in 
+    assume(Log idp authnReq);
   	let authnReqest = SamlProtocolMessage idp authnReq sigSP "relay" in 
   	send client authnReqest; (*2*)
   	let authResponse = recieve client in (*7*)
@@ -20,9 +21,8 @@ let serviceprovider me client idp =
   	| SamlProtocolMessage (sp, message, sigIDP, relay) -> 
   		let resource = Resource uri in
   		send client resource	(*8*)
-  	| _ ->  ()
-  | _ -> ()
-
-  ()
+  	| _ ->  send client (Failed (403))(*8.1*)     
+  | _ -> send client (Failed (400))(*2.1*)
+  
 
 end (* Serviceprovider *)
