main.fst
@@ -5,5 +5,6 @@ open Client
 val main: sp:prin -> res:uri -> user:string -> password:string -> unit
 let main sp resource user password = 
 	let req = HttpGet resource in
-		client sp req user password
+		let message = client sp req user password in
+		()
 end
