client.fst
@@ -7,28 +7,27 @@ open Protocol
 - Add asserts
   *)
 
-val client: sp:prin -> req:message -> user:string -> password:string -> unit
+val client: sp:prin -> req:message -> user:string -> password:string -> message
 let client sp req user password = 
     let _ = send sp req in(*1*)
       let res = recieve sp in(*2*)
         match res with
         | SamlProtocolMessage (idp, authnRequest, sigSP, relayState) -> 
           let samlAuthnReq = SamlProtocolMessage idp authnRequest sigSP relayState in
-              send idp samlAuthnReq;
-              let chal = recieve idp in (*4*)
-              match chal with
-              | Challenge (challenge) -> 
-                  let authUserReq = Credentials user password challenge in (*5*)
-                  send idp authUserReq; (*5*)
-                  let idpResp = recieve idp in
-                  match idpResp with
-                  | SamlProtocolMessage (sp', samlResponse, sigIDP, relayState') -> 
-                    let samlResponseRequest =  SamlProtocolMessage sp' samlResponse sigIDP relayState' in (*7*)
-                    send sp' samlResponseRequest;
-                    let resource = recieve sp' in(*8*)
-                    ()
-                  | _ -> ()
-              | _ -> ()
-        | _ -> ()
+          send idp samlAuthnReq;
+          let chal = recieve idp in (*4*)
+          match chal with
+          | Challenge (challenge) -> 
+            let authUserReq = Credentials user password challenge in (*5*)
+            send idp authUserReq; (*5*)
+            let idpResp = recieve idp in
+            match idpResp with
+            | SamlProtocolMessage (sp', samlResponse, sigIDP, relayState') -> 
+              let samlResponseRequest =  SamlProtocolMessage sp' samlResponse sigIDP relayState' in (*7*)
+              send sp' samlResponseRequest;
+              recieve sp' (*8*)
+            | _ -> idpResp (*Report response back to caller*)
+          | _ -> chal (*Report response back to caller*)
+        | _ -> res (*Report response back to caller*)
 
 end (*Client*)
