identityprovider.fst
@@ -12,17 +12,22 @@ let identityprovider me client serviceprovider =
 	let authRequest = recieve client in (*3*)
 	match authRequest with
 	| SamlProtocolMessage (idp, message, sigSP, relay)-> 
-    let challenge = createChallenge client in
+    (*assert (Log serviceprovider message);*)
+    let challenge = CreateChallenge client in
     let challengeMessage = Challenge challenge in
     send client challengeMessage; (*4*)
     let credentials = recieve client in (*5*)
       match credentials with
       | Credentials(user, password, challenge') -> 
-        let (samlresponse, sigIDP) = createSamlResponse me serviceprovider in
+        (*Check credentials and challenge*)
+        let (samlresponse, sigIDP) = CreateSamlResponse me serviceprovider Success in
         let response = SamlProtocolMessage serviceprovider samlresponse sigIDP relay in
         send client response(*6*)
-      | _ -> ()
-	| _ -> ()
-()
+      | _ -> send client (Failed (400))(*6.3*)
+	| _ -> 
+    let (samlresponse, sigIDP) = CreateSamlResponse me serviceprovider Requester in
+    let response = SamlProtocolMessage serviceprovider samlresponse sigIDP relay in
+    send client response(*4.1*)
+  ()
 
 end (*Identityprovider*)
